cleaning

mall.v
@@ -1,17 +1,11 @@
 Require Import CMorphisms.
-Require Import Lia.
 Require Import PeanoNat.
+Require Import Lia.
 
+Require Import wf_nat_more.
 Require Import List_more.
 Require Import List_Type_more.
-Require Import wf_nat_more.
 
-Require Import List_more2.
-
-Require Import List_nat.
-Require Import Fun_nat.
-Require Import misc.
-Require Import Perm.
 Require Import Perm_R_more.
 
 
@@ -25,8 +19,8 @@ Inductive formulas : Set :=
 
 Fixpoint fsize A :=
   match A with
-  | var X => 0
-  | covar X => 0
+  | var X => 1
+  | covar X => 1
   | tens A B => S (fsize A + fsize B)
   | parr A B => S (fsize A + fsize B)
   | aplus A B => S (fsize A + fsize B)
@@ -49,21 +43,23 @@ Proof. now induction A; simpl; try rewrite IHA1; try rewrite IHA2. Qed.
 Lemma fsize_dual : forall A, fsize (dual A) = fsize A.
 Proof. now induction A; simpl; try rewrite IHA1; try rewrite IHA2; try lia. Qed.
 
-Inductive mll : list formulas -> Type :=
-| ax_r : forall X, mll (covar X :: var X :: nil)
-| ex_r : forall l1 l2, mll l1 -> l1 ~~ l2 -> mll l2
-| tens_r : forall A B l1 l2, mll (A :: l1) -> mll (B :: l2) -> mll (tens A B :: l1 ++ l2)
-| parr_r : forall A B l, mll (A :: B :: l) -> mll (parr A B :: l)
-| plus_r1 : forall A B l, mll (A :: l) -> mll (aplus A B :: l)
-| plus_r2 : forall A B l, mll (B :: l) -> mll (aplus A B :: l)
-| with_r : forall A B l, mll (A :: l) -> mll (B :: l) ->  mll (awith A B :: l).
+Ltac fsize_lia := simpl; rewrite ? fsize_dual; lia.
 
-Global Instance Perm_R_mll : Proper (@Perm_R formulas ==> arrow) mll.
+Inductive mall : list formulas -> Type :=
+| ax_r : forall X, mall (covar X :: var X :: nil)
+| ex_r : forall l1 l2, mall l1 -> l1 ~~ l2 -> mall l2
+| tens_r : forall A B l1 l2, mall (A :: l1) -> mall (B :: l2) -> mall (tens A B :: l1 ++ l2)
+| parr_r : forall A B l, mall (A :: B :: l) -> mall (parr A B :: l)
+| plus_r1 : forall A B l, mall (A :: l) -> mall (aplus A B :: l)
+| plus_r2 : forall A B l, mall (B :: l) -> mall (aplus A B :: l)
+| with_r : forall A B l, mall (A :: l) -> mall (B :: l) ->  mall (awith A B :: l).
+
+Global Instance Perm_R_mall : Proper (@Perm_R formulas ==> arrow) mall.
 Proof. now intros l1 l2 Hp pi; apply ex_r with l1. Defined.
 
-Fixpoint psize {l} (pi : mll l) :=
+Fixpoint psize {l} (pi : mall l) :=
   match pi with
-  | ax_r _ => 0
+  | ax_r _ => 1
   | ex_r _ _ pi _ => S (psize pi)
   | tens_r _ _ _ _ pi1 pi2 => S (psize pi1 + psize pi2)
   | parr_r _ _ _ pi => S (psize pi)
@@ -72,193 +68,177 @@ Fixpoint psize {l} (pi : mll l) :=
   | with_r _ _ _ pi1 pi2 => S (psize pi1 + psize pi2)
   end.
 
-Ltac fsize_lia := simpl; rewrite ? fsize_dual; lia.
-
 Lemma cut_admissible : forall A l1 l2,
-  mll (dual A :: l1) -> mll (A :: l2) -> mll (l1 ++ l2).
+  mall (dual A :: l1) -> mall (A :: l2) -> mall (l1 ++ l2).
 Proof with try assumption; try reflexivity; try fsize_lia.
-  enough (forall c s A l0 l1 l2 (pi1 : mll (dual A :: l0)) (pi2 : mll (l1 ++ A :: l2)),
-          s = psize pi1 + psize pi2 -> fsize A <= c -> mll (l1 ++ l0 ++ l2)) as IH.
-  { intros A l1 l2 pi1 pi2.
-    rewrite <- (app_nil_l _) in pi2.
-    refine (IH _ _ A _ _ _ pi1 pi2 _ _)... }
+  enough (forall c s A l0 l1 l2 (pi1 : mall (dual A :: l0)) (pi2 : mall (l1 ++ A :: l2)),
+          s = psize pi1 + psize pi2 -> fsize A <= c -> mall (l1 ++ l0 ++ l2)) as IH
+    by (now intros A l1 l2 pi1 pi2; rewrite <- (app_nil_l _) in pi2; refine (IH _ _ A _ _ _ pi1 pi2 _ _)).
   induction c as [c IHcut0] using lt_wf_rect.
   assert (forall A, fsize A < c -> forall l0 l1 l2,
-                    mll (dual A :: l0) -> mll (l1 ++ A :: l2) -> mll (l1 ++ l0 ++ l2)) as IHcut
+                    mall (dual A :: l0) -> mall (l1 ++ A :: l2) -> mall (l1 ++ l0 ++ l2)) as IHcut
     by (now intros A Hs l0 l1 l2 pi1 pi2 ; refine (IHcut0 _ _ _ _ _ _ _ pi1 pi2 _ _); try eassumption);
     clear IHcut0.
   induction s as [s IHsize0] using lt_wf_rect.
-  assert (forall A l0 l1 l2 (pi1 : mll (dual A :: l0)) (pi2 : mll (l1 ++ A :: l2)),
-            psize pi1 + psize pi2 < s -> fsize A <= c -> mll (l1 ++ l0 ++ l2))
-    as IHsize by (now intros ; eapply IHsize0 ; try eassumption) ; clear IHsize0.
-  intros A l0 l1 l2 pi1 pi2 Heqs Hc.
-  rewrite_all Heqs; clear s Heqs.
+  assert (forall A l0 l1 l2 (pi1 : mall (dual A :: l0)) (pi2 : mall (l1 ++ A :: l2)),
+            psize pi1 + psize pi2 < s -> fsize A <= c -> mall (l1 ++ l0 ++ l2)) as IHsize
+    by (now intros ; eapply IHsize0 ; try eassumption) ; clear IHsize0.
+  intros A l0 l1 l2 pi1 pi2 Heqs Hc; rewrite_all Heqs; clear s Heqs.
   remember (l1 ++ A :: l2) as l ; destruct pi2.
   - (* ax_r *)
     destruct l1 ; inversion Heql ; subst.
-    + simpl; clear - pi1; revert pi1.
-      refine (Perm_R_mll _ _ (Perm_R_cons_append _ _)). (* should be a rewrite Per_R_cons_append, but Coq bug *)
+    + simpl; clear - pi1; revert pi1; refine (Perm_R_mall _ _ (Perm_R_cons_append _ _)).
+        (* could be a rewrite Perm_R_cons_append, but Coq bug *)
     + unit_vs_elt_inv H1; list_simpl...
   - (* ex_r *)
     simpl in IHsize; rewrite Heql in p.
-    destruct (Perm_R_vs_elt_inv _ _ _ _ p) as [[p1 p2] Heq] ; simpl in Heq ; subst.
+    destruct (Perm_R_vs_elt_inv _ _ _ _ p) as [[p1 p2] Heq]; simpl in Heq; subst.
     apply ex_r with (p1 ++ l0 ++ p2);
     [ | now apply Perm_R_app_inv in p; apply Perm_R_app_middle ].
     refine (IHsize _ _ _ _ pi1 pi2 _ _)...
   - (* tens_r *)
     destruct l1 ; inversion Heql ; subst ; simpl in Hc; list_simpl.
     + (* main case *)
-      remember (dual (tens A0 B) :: l0) as l' ; destruct pi1; try inversion Heql'.
+      remember (dual (tens A0 B) :: l0) as l' ; destruct pi1; inversion Heql'.
       * (* ex_r *)
-        remember (tens_r _ _ _ _ pi2_1 pi2_2) as Htens ; clear HeqHtens.
-        revert p IHsize; rewrite Heql'; change (dual (tens A0 B) :: l0)
-                                          with (nil ++ (dual (tens A0 B) :: l0)); intros p IHsize.
-        destruct (Perm_R_vs_cons_inv _ _ _ p) as [[p1 p2] Heq] ; simpl in Heq; subst.
+        remember (tens_r _ _ _ _ pi2_1 pi2_2) as Htens; clear HeqHtens.
+        revert p IHsize; rewrite Heql'; rewrite <- (app_nil_l (dual (tens A0 B) :: _)); intros p IHsize.
+        destruct (Perm_R_vs_cons_inv _ _ _ p) as [[p1 p2] Heq]; simpl in Heq; subst.
         apply ex_r with (p1 ++ (l3 ++ l4) ++ p2);
         [ | clear - p; apply Perm_R_app_inv in p; simpl in p; rewrite <- p; list_simpl;
             apply Perm_R_app_head; now rewrite (Perm_R_app_comm p2); list_simpl ].
         revert Htens IHsize ; simpl;
-          replace (tens A0 B) with (dual (parr (dual A0) (dual B))) by (now simpl ; rewrite 2 bidual) ;
+          replace (tens A0 B) with (dual (parr (dual A0) (dual B))) by (now simpl; rewrite 2 bidual);
           intros Htens IHsize.
         refine (IHsize _ _ _ _ Htens pi1 _ _)...
       * (* parr_r *)
-        clear IHsize ; subst.
-        rewrite <- (bidual A0) in pi2_1; rewrite <- (bidual B) in pi2_2.
-        refine (IHcut _ _ _ _ _ pi2_1 _)...
+        clear IHsize; subst.
+        rewrite <- (bidual A0) in pi2_1; refine (IHcut _ _ _ _ _ pi2_1 _)...
         apply ex_r with ((dual A0 :: nil) ++ l4 ++ l0); [ | now rewrite <- Perm_R_app_rot ].
-          (* should be a rewrite Per_R_cons_append, but Coq bug *)
-        refine (IHcut _ _ _ _ _ pi2_2 _)...
+          (* could be done with rewrite, but Coq bug *)
+        rewrite <- (bidual B) in pi2_2; refine (IHcut _ _ _ _ _ pi2_2 _)...
     + (* commutative case *)
       dichot_Type_elt_app_exec H1 ; subst.
-      * rewrite 2 app_assoc ; apply tens_r...
-        revert pi2_1 IHsize ; simpl ; rewrite (app_comm_cons _ _ A0) ; intros pi2_1 IHsize; list_simpl.
+      * rewrite 2 app_assoc; apply tens_r...
+        revert pi2_1 IHsize ; simpl ; rewrite (app_comm_cons _ _ A0); intros pi2_1 IHsize; list_simpl.
         refine (IHsize _ _ _ _ pi1 pi2_1 _ _)...
       * list_simpl ; apply tens_r...
-        revert pi2_2 IHsize ; simpl ; rewrite (app_comm_cons _ _ B) ; intros pi2_2 IHsize.
+        revert pi2_2 IHsize; simpl; rewrite (app_comm_cons _ _ B); intros pi2_2 IHsize.
         refine (IHsize _ _ _ _ pi1 pi2_2 _ _)...
   - (* parr_r *)
-    destruct l1 ; inversion Heql; subst; simpl in Hc; list_simpl.
+    destruct l1; inversion Heql; subst; simpl in Hc; list_simpl.
     + (* main case *)
-      remember (dual (parr A0 B) :: l0) as l' ; destruct pi1; try inversion Heql'.
+      remember (dual (parr A0 B) :: l0) as l'; destruct pi1; inversion Heql'.
       * (* ex_r *)
-        remember (parr_r _ _ _ pi2) as Hparr ; clear HeqHparr.
-        revert p IHsize; rewrite Heql'; change (dual (parr A0 B) :: l0)
-                                          with (nil ++ dual (parr A0 B) :: l0); intros p IHsize.
-        destruct (Perm_R_vs_cons_inv _ _ _ p) as [[p1 p2] Heq] ; simpl in Heq ; subst.
+        remember (parr_r _ _ _ pi2) as Hparr; clear HeqHparr.
+        revert p IHsize; rewrite Heql'; rewrite <- (app_nil_l (dual (parr A0 B) :: _)); intros p IHsize.
+        destruct (Perm_R_vs_cons_inv _ _ _ p) as [[p1 p2] Heq]; simpl in Heq; subst.
         apply ex_r with (p1 ++ l2 ++ p2);
         [ | clear - p; apply Perm_R_app_inv in p; simpl in p; rewrite <- p; list_simpl;
             apply Perm_R_app_head, Perm_R_app_comm ].
-        revert Hparr IHsize ; simpl ;
-          replace (parr A0 B) with (dual (tens (dual A0) (dual B)))
-          by (simpl ; rewrite 2 bidual ; reflexivity) ;
+        revert Hparr IHsize; simpl;
+          replace (parr A0 B) with (dual (tens (dual A0) (dual B))) by (now simpl; rewrite 2 bidual);
           intros Hparr IHsize.
         refine (IHsize _ _ _ _ Hparr pi1 _ _)...
       * (* tens_r *)
-        clear IHsize ; subst.
-        rewrite <- (app_nil_l (A0 :: _)) in pi2 ; simpl in Hc ; list_simpl.
-        refine (IHcut _ _ _ _ _ pi1_2 _)...
-        rewrite <- (app_nil_l _) ; refine (IHcut _ _ _ _ _ pi1_1 _)...
+        clear IHsize; subst; list_simpl.
+        rewrite <- (app_nil_l (A0 :: _)) in pi2; refine (IHcut _ _ _ _ _ pi1_2 _)...
+        rewrite <- (app_nil_l _); refine (IHcut _ _ _ _ _ pi1_1 _)...
     + (* commutative case *)
       apply parr_r.
-      revert pi2 IHsize ; simpl ; rewrite (app_comm_cons l1 _ B) ; rewrite (app_comm_cons _ _ A0) ;
-        intros pi2 IHsize.
+      revert pi2 IHsize; simpl; rewrite (app_comm_cons l1 _ B), (app_comm_cons _ _ A0); intros pi2 IHsize.
       refine (IHsize _ _ _ _ pi1 pi2 _ _)...
   - (* plus_r1 *)
     destruct l1; inversion Heql; subst; simpl in Hc; list_simpl.
     + (* main case *)
-      remember (dual (aplus A0 B) :: l0) as l' ; destruct pi1; try inversion Heql'.
+      remember (dual (aplus A0 B) :: l0) as l'; destruct pi1; inversion Heql'.
       * (* ex_r *)
-        remember (plus_r1 _ _ _ pi2) as Hplus ; clear HeqHplus.
-        revert p IHsize; rewrite Heql'; change (dual (aplus A0 B) :: l0)
-                                          with (nil ++ (dual (aplus A0 B)) :: l0); intros p IHsize.
-        destruct (Perm_R_vs_cons_inv _ _ _ p) as [[p1 p2] Heq] ; simpl in Heq ; subst.
+        remember (plus_r1 _ _ _ pi2) as Hplus; clear HeqHplus.
+        revert p IHsize; rewrite Heql'; rewrite <- (app_nil_l (dual (aplus A0 B) :: _)); intros p IHsize.
+        destruct (Perm_R_vs_cons_inv _ _ _ p) as [[p1 p2] Heq]; simpl in Heq; subst.
         apply ex_r with (p1 ++ l2 ++ p2);
         [ | clear - p; apply Perm_R_app_inv in p; simpl in p; rewrite <- p; list_simpl;
             apply Perm_R_app_head, Perm_R_app_comm ].
-        revert Hplus IHsize ; simpl ;
-          replace (aplus A0 B) with (dual (awith (dual A0) (dual B)))
-          by (simpl ; rewrite 2 bidual ; reflexivity) ;
+        revert Hplus IHsize; simpl;
+          replace (aplus A0 B) with (dual (awith (dual A0) (dual B))) by (now simpl; rewrite 2 bidual);
           intros Hplus IHsize.
         refine (IHsize _ _ _ _ Hplus pi1 _ _)...
       * (* with_r *)
-        clear IHsize ; subst.
-        rewrite <- (app_nil_l (A0 :: _)) in pi2 ; refine (IHcut _ _ _ _ _ pi1_1 pi2)...
+        clear IHsize; subst.
+        rewrite <- (app_nil_l (A0 :: _)) in pi2; refine (IHcut _ _ _ _ _ pi1_1 pi2)...
     + (* commutative case *)
       apply plus_r1.
-      revert pi2 IHsize ; simpl ; rewrite (app_comm_cons l1 _ A0) ; intros pi2 IHsize.
+      revert pi2 IHsize; simpl; rewrite (app_comm_cons l1 _ A0); intros pi2 IHsize.
       refine (IHsize _ _ _ _ pi1 pi2 _ _)...
   - (* plus_r2 *)
     destruct l1; inversion Heql; subst; simpl in Hc; list_simpl.
     + (* main case *)
-      remember (dual (aplus A0 B) :: l0) as l' ; destruct pi1; try inversion Heql'.
+      remember (dual (aplus A0 B) :: l0) as l'; destruct pi1; inversion Heql'.
       * (* ex_r *)
-        remember (plus_r2 _ _ _ pi2) as Hplus ; clear HeqHplus.
-        revert p IHsize; rewrite Heql'; rewrite<- (app_nil_l (dual (aplus A0 B) :: l0)); intros p IHsize.
-        destruct (Perm_R_vs_cons_inv _ _ _ p) as [[p1 p2] Heq] ; simpl in Heq; subst.
+        remember (plus_r2 _ _ _ pi2) as Hplus; clear HeqHplus.
+        revert p IHsize; rewrite Heql'; rewrite <- (app_nil_l (dual (aplus A0 B) :: l0)); intros p IHsize.
+        destruct (Perm_R_vs_cons_inv _ _ _ p) as [[p1 p2] Heq]; simpl in Heq; subst.
         apply ex_r with (p1 ++ l2 ++ p2);
         [ | clear - p; apply Perm_R_app_inv in p; simpl in p; rewrite <- p; list_simpl;
             apply Perm_R_app_head, Perm_R_app_comm ].
-        revert Hplus IHsize ; simpl ;
-          replace (aplus A0 B) with (dual (awith (dual A0) (dual B)))
-          by (simpl ; rewrite 2 bidual ; reflexivity) ;
+        revert Hplus IHsize; simpl;
+          replace (aplus A0 B) with (dual (awith (dual A0) (dual B))) by (now simpl; rewrite 2 bidual);
           intros Hplus IHsize.
         refine (IHsize _ _ _ _ Hplus pi1 _ _)...
       * (* with_r *)
-        clear IHsize ; subst.
-        rewrite <- (app_nil_l (B :: _)) in pi2 ; refine (IHcut _ _ _ _ _ pi1_2 pi2)...
+        clear IHsize; subst.
+        rewrite <- (app_nil_l (B :: _)) in pi2; refine (IHcut _ _ _ _ _ pi1_2 pi2)...
     + (* commutative case *)
       apply plus_r2.
-      revert pi2 IHsize ; simpl ; rewrite (app_comm_cons l1 _ B) ; intros pi2 IHsize.
+      revert pi2 IHsize; simpl; rewrite (app_comm_cons l1 _ B); intros pi2 IHsize.
       refine (IHsize _ _ _ _ pi1 pi2 _ _)...
   - (* with_r *)
     destruct l1; inversion Heql; subst; simpl in Hc; list_simpl.
     + (* main case *)
-      remember (dual (awith A0 B) :: l0) as l' ; destruct pi1 ; try inversion Heql'.
+      remember (dual (awith A0 B) :: l0) as l'; destruct pi1; inversion Heql'.
       * (* ex_r *)
-        remember (with_r _ _ _ pi2_1 pi2_2) as Hwith ; clear HeqHwith.
-        revert p IHsize; rewrite Heql'; change (dual (awith A0 B) :: l0)
-                                          with (nil ++ dual (awith A0 B) :: l0); intros p IHsize.
-        destruct (Perm_R_vs_cons_inv _ _ _ p) as [[p1 p2] Heq] ; simpl in Heq ; subst.
+        remember (with_r _ _ _ pi2_1 pi2_2) as Hwith; clear HeqHwith.
+        revert p IHsize; rewrite Heql'; rewrite <- (app_nil_l (dual (awith A0 B) :: _)); intros p IHsize.
+        destruct (Perm_R_vs_cons_inv _ _ _ p) as [[p1 p2] Heq]; simpl in Heq; subst.
         apply ex_r with (p1 ++ l2 ++ p2);
         [ | clear - p; apply Perm_R_app_inv in p; simpl in p; rewrite <- p; list_simpl;
             apply Perm_R_app_head, Perm_R_app_comm ].
         revert Hwith IHsize ; simpl ;
-          replace (awith A0 B) with (dual (aplus (dual A0) (dual B)))
-          by (simpl ; rewrite 2 bidual ; reflexivity) ;
+          replace (awith A0 B) with (dual (aplus (dual A0) (dual B))) by (now simpl; rewrite 2 bidual);
           intros Hwith IHsize.
         refine (IHsize _ _ _ _ Hwith pi1 _ _)...
       * (* plus_r1 *)
-        clear IHsize ; subst.
+        clear IHsize; subst.
         rewrite <- (app_nil_l (A0 :: _)) in pi2_1; refine (IHcut _ _ _ _ _ pi1 pi2_1)...
       * (* plus_r2 *)
-        clear IHsize ; subst.
+        clear IHsize; subst.
         rewrite <- (app_nil_l (B :: _)) in pi2_2 ; refine (IHcut _ _ _ _ _ pi1 pi2_2)...
     + (* commutative case *)
       apply with_r.
-      * revert pi2_1 IHsize ; simpl ; rewrite (app_comm_cons l1 _ A0) ; intros pi2_1 IHsize.
+      * revert pi2_1 IHsize; simpl; rewrite (app_comm_cons l1 _ A0); intros pi2_1 IHsize.
         refine (IHsize _ _ _ _ pi1 pi2_1 _ _)...
-      * revert pi2_2 IHsize ; simpl ; rewrite (app_comm_cons l1 _ B) ; intros pi2_2 IHsize.
+      * revert pi2_2 IHsize; simpl; rewrite (app_comm_cons l1 _ B); intros pi2_2 IHsize.
         refine (IHsize _ _ _ _ pi1 pi2_2 _ _)...
 Qed.
 
 
-Inductive mll_cut : list formulas -> Type :=
-| ax_cut_r : forall X, mll_cut (covar X :: var X :: nil)
-| ex_cut_r : forall l1 l2, mll_cut l1 -> l1 ~~ l2 -> mll_cut l2
-| tens_cut_r : forall A B l1 l2, mll_cut (A :: l1) -> mll_cut (B :: l2) -> mll_cut (tens A B :: l1 ++ l2)
-| parr_cut_r : forall A B l, mll_cut (A :: B :: l) -> mll_cut (parr A B :: l)
-| plus_cut_r1 : forall A B l, mll_cut (A :: l) -> mll_cut (aplus A B :: l)
-| plus_cut_r2 : forall A B l, mll_cut (B :: l) -> mll_cut (aplus A B :: l)
-| with_cut_r : forall A B l, mll_cut (A :: l) -> mll_cut (B :: l) -> mll_cut (awith A B :: l)
-| cut_r : forall A l1 l2, mll_cut (dual A :: l1) -> mll_cut (A :: l2) ->  mll_cut (l1 ++ l2).
+Inductive mall_cut : list formulas -> Type :=
+| ax_cut_r : forall X, mall_cut (covar X :: var X :: nil)
+| ex_cut_r : forall l1 l2, mall_cut l1 -> l1 ~~ l2 -> mall_cut l2
+| tens_cut_r : forall A B l1 l2, mall_cut (A :: l1) -> mall_cut (B :: l2) -> mall_cut (tens A B :: l1 ++ l2)
+| parr_cut_r : forall A B l, mall_cut (A :: B :: l) -> mall_cut (parr A B :: l)
+| plus_cut_r1 : forall A B l, mall_cut (A :: l) -> mall_cut (aplus A B :: l)
+| plus_cut_r2 : forall A B l, mall_cut (B :: l) -> mall_cut (aplus A B :: l)
+| with_cut_r : forall A B l, mall_cut (A :: l) -> mall_cut (B :: l) -> mall_cut (awith A B :: l)
+| cut_r : forall A l1 l2, mall_cut (dual A :: l1) -> mall_cut (A :: l2) ->  mall_cut (l1 ++ l2).
 
-Global Instance Perm_R_mll_cut : Proper (@Perm_R formulas ==> arrow) mll_cut.
+Global Instance Perm_R_mall_cut : Proper (@Perm_R formulas ==> arrow) mall_cut.
 Proof. now intros l1 l2 Hp pi; apply ex_cut_r with l1. Defined.
 
-Theorem cut_elim : forall l, mll_cut l -> mll l.
+Theorem cut_elim : forall l, mall_cut l -> mall l.
 Proof.
-  intros l pi.
-  induction pi; try (now constructor); try (eapply ex_r; eassumption).
-  now apply cut_admissible with A.
+  intros l pi; induction pi; try now constructor.
+  - now apply ex_r with l1.
+  - now apply cut_admissible with A.
 Qed.
 
